Complete Homework 2.4 #5(b)

LogicFormalization/Chapter2/Section4/Homework.lean
@@ -1,6 +1,7 @@
 import LogicFormalization.Chapter2.Section4.Term
 import Mathlib.Data.Fin.VecNotation
 import Mathlib.Tactic.Linarith.Frontend
+import Mathlib.Tactic.Ring
 
 namespace Homeworks
 
@@ -105,10 +106,161 @@ theorem not_exists_nat_rig_term₁ : ¬∃ (t: Term .Rig) (x: Var) (hx: AreVarsF
 end a
 
 
+section b
+
+/-- Represents polynomials with coefficients from `ℕ`.-/
+inductive Poly
+| const: ℕ → Poly
+| var
+| add: Poly → Poly → Poly
+| mul: Poly → Poly → Poly
+
+namespace Poly
+
+def eval: Poly → ℕ → ℕ
+| .const a, _ => a
+| .var, n => n
+| .add p q, n => p.eval n + q.eval n
+| .mul p q, n => p.eval n * q.eval n
+
+lemma eval_mono: ∀ {p: Poly}, Monotone p.eval
+| .const _ => fun _ _ _ => Nat.le_refl _
+| .var => fun _ _ => id
+| .add _ _ => Monotone.add eval_mono eval_mono
+| .mul _
+ _ => Monotone.mul' eval_mono eval_mono
+
+/-- Degree of a polynomial -/
+def deg: Poly → ℕ
+| .const _ => 0
+| .var => 1
+| .add p q => max (deg p) (deg q)
+| .mul p q => deg p + deg q
+
+/-- Polynomials are homogenous. -/
+lemma eval_mul_le {a n} (ha: a ≠ 0) : ∀ {p: Poly}, eval p (a * n) ≤ a^(deg p) * eval p n
+| .const c | .var => by simp [eval, deg]
+| .add q r => calc eval (add q r) (a * n)
+  _ = eval q (a * n) + eval r (a * n) := rfl
+  _ ≤ a^(deg q) * eval q n + a^(deg r) * eval r n :=
+    Nat.add_le_add (eval_mul_le ha) (eval_mul_le ha)
+  _ ≤ _ := by
+    apply (Nat.le_or_ge (deg q) (deg r)).elim
+    · intro h
+      simp only [deg, h, sup_of_le_right, eval, Nat.mul_add, add_le_add_iff_right]
+      apply Nat.mul_le_mul_right
+      apply Nat.pow_le_pow_right <;> simp [*, Nat.zero_lt_of_ne_zero]
+    · intro h
+      simp only [deg, h, sup_of_le_left, eval, Nat.mul_add, add_le_add_iff_left]
+      apply Nat.mul_le_mul_right
+      apply Nat.pow_le_pow_right <;> simp [*, Nat.zero_lt_of_ne_zero]
+| .mul q r => calc eval (mul q r) (a * n)
+  _ = eval q (a * n) * eval r (a * n) := rfl
+  _ ≤ (a^(deg q) * eval q n) * (a^(deg r) * eval r n) :=
+    Nat.mul_le_mul (eval_mul_le ha) (eval_mul_le ha)
+  _ = _ := by simp [deg, eval]; ring
+
+/-- Roughly speaking, use `eval_mul_le` to go from `p(n)`
+to `p(2 * n / 2)` to `2^deg(p) p(n)`. This is complicated
+by the fact that we are in `ℕ` and lack clean division.
+We end up using `⌈n/2⌉` instead. -/
+lemma eval_le_mul_eval_half {p: Poly} {n: ℕ}:
+    eval p n ≤ 2^(deg p) * eval p ((n + 1) / 2) := calc _
+  _ ≤ eval p (2 * ((n + 1) / 2)) := eval_mono (by omega)
+  _ ≤ _ := eval_mul_le (by decide)
+
+/-- p(n) does not converge to 2^n as n → ∞ -/
+lemma eval_diverges_from_two_pow: ∀ p m, ∃ N, ∀ n ≥ N, m * eval p n < 2^n
+| .const c, m => ⟨m * c, fun n hn => Nat.lt_of_le_of_lt hn Nat.lt_two_pow_self⟩
+| .var, m => ⟨m + 1, fun n hn =>
+  have: m ≤ n - 1 := Nat.le_sub_one_of_lt hn
+  Nat.lt_of_le_of_lt
+    (Nat.mul_le_mul_right n this) mul_pred_self_lt_two_pow⟩
+| .add q r, m =>
+  let ⟨Nq, hq⟩ := eval_diverges_from_two_pow q (2 * m)
+  let ⟨Nr, hr⟩ := eval_diverges_from_two_pow r (2 * m)
+  ⟨max Nq Nr, fun n hn => by
+    replace hu := hq n (le_of_max_le_left hn)
+    replace hv := hr n (le_of_max_le_right hn)
+    have := Nat.add_lt_add hu hv
+    simp_rw [Nat.two_mul, Nat.add_mul, ←Nat.two_mul, ←Nat.mul_add] at this
+    exact Nat.lt_of_mul_lt_mul_left this⟩
+| .mul q r, m =>
+  -- this one is trickier. we make use of the homogeneity property (`eval_mul_le`)
+  let ⟨Nq, hq⟩ := eval_diverges_from_two_pow q (m * 2^(deg q))
+  let ⟨Nr, hr⟩ := eval_diverges_from_two_pow r (2 * 2^(deg r))
+  ⟨(max Nq Nr) * 2, fun n hn => by
+    replace hq := hq ((n + 1) / 2) (by omega)
+    replace hr := hr ((n + 1) / 2) (by omega)
+    replace hr: 2 ^ r.deg * r.eval ((n + 1) / 2) < 2 ^ ((n + 1) / 2 - 1) := by
+      simp only [Nat.mul_assoc] at hr
+      apply Nat.lt_of_mul_lt_mul_left (a := 2)
+      rw [←Nat.pow_succ']
+      apply Nat.lt_of_lt_of_le hr
+      apply Nat.pow_le_pow_right (by decide)
+      omega
+
+    calc m * eval (mul q r) n
+      _ = m * (eval q n * eval r n) := rfl
+      _ ≤ m * ((2^(deg q) * eval q ((n + 1) / 2)) * (2^(deg r) * eval r ((n + 1) / 2))) := by
+        apply Nat.mul_le_mul_left
+        apply Nat.mul_le_mul <;> exact eval_le_mul_eval_half
+      _ = (m * 2^(deg q) * eval q ((n + 1) / 2)) * (2^(deg r) * eval r ((n + 1) / 2)) := by ring
+      _ < (2 ^ ((n + 1) / 2)) * (2 ^ ((n + 1) / 2 - 1)) := Nat.mul_lt_mul'' hq hr
+      _ = 2 ^ ((n + 1) / 2 + ((n + 1) / 2 - 1)) := (Nat.pow_add ..).symm
+      _ ≤ 2 ^ n := Nat.pow_le_pow_right (by decide) (by omega)⟩
+where
+  mul_pred_self_lt_two_pow : ∀ {n: ℕ}, (n - 1) * n < 2^n
+  | 0 => by decide
+  | k + 1 => calc (k + 1 - 1) * (k + 1)
+    _ = k * (k + 1) := rfl
+    _ = (k - 1) * k + 2 * k := by
+      simp only [Nat.mul_succ, Nat.sub_mul]
+      have := Nat.sub_add_cancel (Nat.le_mul_self k)
+      omega
+    _ < 2 ^ k + 2 * k :=
+      Nat.add_lt_add_right mul_pred_self_lt_two_pow _
+    _ ≤ 2 ^ (k + 1) := by
+      simp only [Nat.pow_succ, Nat.mul_two, add_le_add_iff_left]
+      have: (k - 1) + 1 ≤ 2^(k-1) := Nat.lt_two_pow_self
+      match k with
+      | 0 => decide
+      | l + 1 =>
+        rw [Nat.add_sub_cancel] at this
+        omega
+
+/-- Convert one of the `L`-terms to a `Poly`. -/
+def ofTerm (t: Term .Rig) {x: Var} (hx: AreVarsFor ![x] t):
+    { p // ∀ n, interp t 𝒩 hx ![n] = eval p n } :=
+  match t with
+  | .var _ => ⟨.var, fun n => by simp [interp, eval]⟩
+  | .app .zero _ => ⟨.const 0, fun n => rfl⟩
+  | .app .one _ => ⟨.const 1, fun n => rfl⟩
+  | .app .add ts =>
+    let ⟨a, ha⟩ := ofTerm (ts 0) (.ofApp hx 0)
+    let ⟨b, hb⟩ := ofTerm (ts 1) (.ofApp hx 1)
+    ⟨.add a b, fun n => by simp only [eval, ←ha, ←hb]; rfl⟩
+  | .app .mul ts =>
+    let ⟨a, ha⟩ := ofTerm (ts 0) (.ofApp hx 0)
+    let ⟨b, hb⟩ := ofTerm (ts 1) (.ofApp hx 1)
+    ⟨.mul a b, fun n => by simp only [eval, ←ha, ←hb]; rfl⟩
+
+end Poly
+
+
 /-- 2.4 #5 (b) -/
 theorem not_exists_nat_rig_term₂ : ¬∃ (t: Term .Rig) (x: Var) (hx: AreVarsFor ![x] t),
     ∀ n, interp t 𝒩 hx ![n] = 2^n :=
-  sorry
+  fun ⟨t, x, hx, h⟩ =>
+    let ⟨p, hp⟩ := Poly.ofTerm t hx
+    have ⟨N, hN⟩ := Poly.eval_diverges_from_two_pow p 17
+    by {
+      have := hN N (Nat.le_refl N)
+      rw [←h N, hp N] at this
+      omega
+    }
+
+end b
 
 open Structure in
 /-- 2.4 #5 (c). The only substructure of `𝒩` is `𝒩` itself. -/
